LateX Equations (for Tom's Model):
$S_h = -\lambda_h N_{sy}+1-\alpha N_{sy} (\iota)+1-\omega_a \mu_a N_{ih}-\mu_a N_{sh}$
$S_l = -\lambda_l N_{sl}+1-\alpha*N_{sy}*(\iota)+1-\omega_a \mu_a N_{il}-\mu_a N_{sh}$
$S_y = -\lambda_y N_{sy}+1-\alpha N_{sy} (\iota)+1-\omega_y N_{sh}$

$A_h = -\lambda_h N_{sy}+1-\alpha*N_{sy}*(\iota)+1-\omega_a \mu_a*N_h-\mu_a*N_{sh}$
$A_l = -\lambda_l*N_{sl}+1-\alpha*N_{sy}*(\iota)+1-\omega_a*\mu_a*N_h-\mu_a*N_{sh}$
$A_y = -\lambda_y*N_{sy}+1-\alpha*N_{sy}*(\iota)+1-\omega_y*N_{sh}$

$I_h = -\lambda_h N_{sy}+1-\alpha*N_{sy}*(\iota)+1-\omega_a \mu_a*N_h-\mu_a*N_{sh}$
$I_l = -\lambda_l*N_{sl}+1-\alpha*N_{sy}*(\iota)+1-\omega_a*\mu_a*N_h-\mu_a*N_{sh}$
$I_y = -\lambda_y*N_{sy}+1-\alpha*N_{sy}*(\iota)+1-\omega_y*N_{sh}$

$R_h = \gamma*N_{ih}+1-\alpha*N_{ry}*(\iota)+1-\mu_a*N_h*N_{rh}$
$R_l = \gamma*N_{il}+1-\alpha*N_{ry}*(\iota)+1-\mu_a*N_h*N_{rl}$
$R_y = \gamma*N_{iy}+1-\alpha*N_{ry}*(\iota)+1-\mu_a*N_h*N_{ry}$

$V_h = \omega_a N_h-\mu_a N_{vh}+1-\omega_y*N_{sy}*\iota$
$V_h = \omega_a N_l-\mu_a N_{vl}+1-\omega_y*N_{sy}*\iota$